tools/examples/simpleTestBenign.ll
@@ -1,0 +1,20 @@
+entry:
+  %cmp = icmp sle i32 %x, 0
+  br i1 %cmp, label %if.then, label %lor.lhs.false
+
+lor.lhs.false:                                    ; preds = %entry
+  %cmp1 = icmp sgt i32 %x, 2
+  br i1 %cmp1, label %if.then, label %if.end
+
+if.then:                                          ; preds = %lor.lhs.false, %entry
+  store i32 0, i32* %retval, align 4
+  br label %return
+
+if.end:                                           ; preds = %lor.lhs.false
+  store i32 %x, i32* %retval, align 4
+  br label %return
+
+return:                                           ; preds = %if.end, %if.then
+  %3 = load i32, i32* %retval, align 4
+  ret i32 %3
+  
