tools/examples/simpleTestPatchBenign.ll
@@ -1,0 +1,3 @@
+entry:
+    ret i32 0
+
