Dafny/examples/Challenge9/Challenge9PropertiesExample.i.dfy
@@ -10,19 +10,121 @@ module challenge9PropertiesExample{
     import opened Collections__Seqs_s
 
 
-lemma isPatchIsSuccesful()
-    ensures forall s,b :: && ValidState(s) 
-                          && validConfig(s) 
-                          && b == [s] + evalCodeFn(entrySimple(),s) ==> !miniSpec(s,b)
-{
-    forall s:State,b | && ValidState(s) && validConfig(s) && b == [s] + evalCodeFn(entrySimple(),s)
-        ensures !miniSpec(s,b);
-     {
-        var b := unwrapPatch(s);
-        assert !miniSpec(s,b);
-     }
-}
+    lemma isPatchIsSuccesful()
+        ensures forall s,b :: && ValidState(s) 
+                            && validConfig(s) 
+                            && b == [s] + evalCodeFn(entrySimple(),s) ==> !miniSpec(s,b)
+    {
+        forall s:State,b | && ValidState(s) && validConfig(s) && b == [s] + evalCodeFn(entrySimple(),s)
+            ensures !miniSpec(s,b);
+        {
+            var b := unwrapPatch(s);
+            assert !miniSpec(s,b);
+        }
+    }
 
+    lemma  vulnAlwaysReturns1()
+        ensures forall s:State,bVuln :: && ValidState(s) 
+                                && validConfig(s) 
+                                && bVuln == [s] + evalCodeFn(entrySimplVuln(),s) ==> OperandContents(last(bVuln),allVariablesConfig().ops["var_28"]).val == 1; 
+    {
+        forall s:State,bVuln | && ValidState(s) 
+                         && validConfig(s) 
+                                && bVuln == [s] + evalCodeFn(entrySimplVuln(),s)
+            ensures OperandContents(last(bVuln),allVariablesConfig().ops["var_28"]).val == 1; 
+        {
+            var b :=  unwrapVuln(s);
+            assert  bVuln == b;
+            assert OperandContents(last(bVuln),allVariablesConfig().ops["var_28"]).val == 1; 
+        }
+    }
+
+    // predicate testVal(b:Behavior)
+    // {
+    //     OperandContents(last(b),allVariablesConfig().ops["var_28"]).val == 1
+    // }
+
+    // predicate badbehavior(s:State,b:Behavior)
+    // {
+    //      OperandContents(last(b),allVariablesConfig().ops["var_0"]).val >= 255 ==> miniSpec(s,b)
+    // }
+
+    // lemma testValImpliesItself(s:State,b:Behavior)
+    // requires ValidState(s) 
+    //     requires validConfig(s) 
+    //     requires b == [s] + evalCodeFn(entrySimplVuln(),s)
+    //     ensures testVal(b) ==> OperandContents(last(b),allVariablesConfig().ops["var_28"]).val == 1;
+    // {
+        
+    // }
+
+    lemma  vulnIs(s:State, b:Behavior)
+        requires ValidState(s) 
+        requires validConfig(s) 
+        requires b == [s] + evalCodeFn(entrySimplVuln(),s)
+               requires ValidOperand(last(b),allVariablesConfig().ops["var_28"])
+       requires OperandContents(last(b),allVariablesConfig().ops["var_28"]).Int?
+       requires ValidOperand(last(b),allVariablesConfig().ops["var_0"])
+       requires OperandContents(last(b),allVariablesConfig().ops["var_0"]).Int?
+        // ensures testVal(b)
+        // ensures badbehavior(s,b)
+        // ensures OperandContents(last(b),allVariablesConfig().ops["var_0"]).val >= 255 ==> miniSpec(s,b);
+    {
+        // vulnAlwaysReturns1();
+        var bVuln := unwrapVuln(s);
+        assert b == bVuln;
+        assert OperandContents(last(b),allVariablesConfig().ops["var_28"]).val == 1;  
+        assert OperandContents(last(b),allVariablesConfig().ops["var_0"]).val >= 255 ==> miniSpec(s,b);
+    }
+
+
+    predicate latest(s:State,a:Behavior,b:Behavior)
+        requires ValidState(s) 
+        requires validConfig(s) 
+    {
+        (a == [s] + evalCodeFn(entrySimplVuln(),s)  
+        && !miniSpec(s,a) 
+        && b == [s] + evalCodeFn(entrySimple(),s)) ==>
+        OperandContents(last(b),allVariablesConfig().ops["var_28"]).val ==OperandContents(last(b),allVariablesConfig().ops["var_28"]).val
+}
+    lemma isPatchIsComplete(s:State)
+        requires ValidState(s) 
+        requires validConfig(s) 
+        ensures forall bVuln,pPAtch :: && bVuln == [s] + evalCodeFn(entrySimplVuln(),s)  
+                                       && !miniSpec(s,bVuln) 
+                                       && pPAtch == [s] + evalCodeFn(entrySimple(),s) ==>
+                                       OperandContents(last(pPAtch),allVariablesConfig().ops["var_28"]).val == OperandContents(last(bVuln),allVariablesConfig().ops["var_28"]).val
+    {
+        forall bVuln |&& bVuln == [s] + evalCodeFn(entrySimplVuln(),s) 
+            ensures !miniSpec(s,bVuln) ==> (OperandContents(last(bVuln),allVariablesConfig().ops["var_0"]).val < 255);
+            ensures OperandContents(last(bVuln),allVariablesConfig().ops["var_28"]).val == 1; 
+        {
+            // var b' := unwrapPatch(s);
+            // var b := unwrapVuln(s);
+            // vulnAlwaysReturns1();
+            var b :=  unwrapVuln(s);
+            assert  bVuln == b;
+            // assert OperandContents(last(bVuln),allVariablesConfig().ops["var_28"]).val == 1; 
+            // assert !miniSpec(s,b) ==> (OperandContents(last(b),allVariablesConfig().ops["var_0"]).val < 255);
+           
+        }
+        forall bVuln,pPAtch |&& bVuln == [s] + evalCodeFn(entrySimplVuln(),s)  && !miniSpec(s,bVuln) 
+        && pPAtch == [s] + evalCodeFn(entrySimple(),s) 
+            ensures OperandContents(last(pPAtch),allVariablesConfig().ops["var_28"]).val ==OperandContents(last(bVuln),allVariablesConfig().ops["var_28"]).val;
+        {
+            var b' := unwrapPatch(s);
+            assert pPAtch == b';
+            // assert OperandContents(last(b'),allVariablesConfig().ops["var_28"]).val == 1; 
+            // assert OperandContents(last(bVuln),allVariablesConfig().ops["var_28"]).val == 1; 
+
+            // assert 
+ 
+        }
+         assert forall bVuln,pPAtch :: && bVuln == [s] + evalCodeFn(entrySimplVuln(),s)  
+                                       && !miniSpec(s,bVuln) 
+                                       && pPAtch == [s] + evalCodeFn(entrySimple(),s) ==>
+                                       OperandContents(last(pPAtch),allVariablesConfig().ops["var_28"]).val ==OperandContents(last(bVuln),allVariablesConfig().ops["var_28"]).val;
+    }
 
     lemma unwrapPatch(s:State) returns (b:Behavior)
         requires ValidState(s);
@@ -50,6 +152,36 @@ lemma isPatchIsSuccesful()
             
             assert (OperandContents(last(b),config.ops["var_0"]).val >= 255 && OperandContents(last(b),config.ops["var_0"]).val < 0x8000_0000) ==> OperandContents(last(b),config.ops["var_28"]).val == 0;
             assert OperandContents(last(b),config.ops["var_0"]).val < 255 ==> OperandContents(last(b),config.ops["var_28"]).val == 1;
+    }
+
+
+    lemma unwrapVuln(s:State) returns (b:Behavior)
+        requires ValidState(s);
+        requires validConfig(s);
+        ensures b == [s] + evalCodeFn(entrySimplVuln(),s);
+        // ensures testVal(b)
+        // ensures !miniSpec(s,b);
+        ensures OperandContents(last(b),allVariablesConfig().ops["var_28"]).val == 1;
+        ensures miniSpec(s,b) ==> (OperandContents(last(b),allVariablesConfig().ops["var_0"]).val >= 255 && OperandContents(last(b),allVariablesConfig().ops["var_0"]).val < 0x8000_0000);
+        ensures !miniSpec(s,b) ==> OperandContents(last(b),allVariablesConfig().ops["var_0"]).val < 255;
+        {
+        var config := allVariablesConfig();
+        b := [s] + evalCodeFn(entrySimplVuln(),s);
+        // assert |b| == 7;
+        assert NextStep(b[0],b[1],evalInsStep((LOAD(config.ops["var_0"],1,config.ops["var_num_connections"]))));
+        assert NextStep(b[1],b[2],evalInsStep((ZEXT(config.ops["var_conv"],1,config.ops["var_0"],4))));
+       
+        assert NextStep(b[2],b[3],evalInsStep((STORE(D(Int(1,IntType(1,false))),config.ops["var_retval"]))));
+
+        
+        assert NextStep(b[3],b[4],evalInsStep((LOAD(config.ops["var_28"],1,config.ops["var_retval"]))));
+        assert NextStep(b[4],b[5],evalInsStep((RET(config.ops["var_28"]))));
+        assert OperandContents(last(b),allVariablesConfig().ops["var_28"]).val == 1;
+                        assert miniSpec(s,b) ==> (OperandContents(last(b),allVariablesConfig().ops["var_0"]).val >= 255 && OperandContents(last(b),allVariablesConfig().ops["var_0"]).val < 0x8000_0000);
+                        assert !miniSpec(s,b) ==> OperandContents(last(b),allVariablesConfig().ops["var_0"]).val < 255;
+
+            // assert (OperandContents(last(b),config.ops["var_0"]).val >= 255 && OperandContents(last(b),config.ops["var_0"]).val < 0x8000_0000) ==> OperandContents(last(b),config.ops["var_28"]).val == 0;
+            // assert OperandContents(last(b),config.ops["var_0"]).val < 255 ==> OperandContents(last(b),config.ops["var_28"]).val == 1;
     }
 
     predicate miniSpec(s:State,b:Behavior)
