Dafny/examples/BenignTest/BenignTestProperties.i.dfy
@@ -1,0 +1,101 @@
+include "simpleTestPatchBenign.i.dfy"
+include "simpleTestBenign.i.dfy"
+include "../../LLVM/llvmNEW.i.dfy"
+include "../../LLVM/types.s.dfy"
+include "../../Libraries/Seqs.s.dfy"
+
+module benignTestProperties{
+    import opened simpleTestPatchBenign
+    import opened simpleTestBenign
+    import opened LLVM_def_NEW
+    import opened types
+    import opened Collections__Seqs_s
+
+
+    lemma unwrapPatch(s:State) returns (b:Behavior)
+        requires ValidState(s);
+        requires validConfigPatch(s);
+        ensures b == [s] + evalCodeFn(entryPatch(),s);
+        ensures last(b).o.o.val == 0;
+    {
+        var config := allVariablesConfigPatch();
+        b := [s] + evalCodeFn(entryPatch(),s);
+        assert |b| == 2;
+        assert last(b).o.o.val == 0;
+    }
+
+    lemma unwrapVuln(s:State) returns (b:Behavior)
+        requires ValidState(s);
+        requires validConfigVuln(s);
+        ensures b == [s] + evalCodeFn(entryVuln(),s);
+        ensures last([s] + evalCodeFn(entryVuln(),s)).o.Out?;
+        ensures last([s] + evalCodeFn(entryVuln(),s)).o.o.Int?;
+        // ensures unwrapVuln(s) == last([s] + evalCodeFn(entryVuln(),s))
+    {
+        var config := allVariablesConfigVuln();
+        b := [s] + evalCodeFn(entryVuln(),s);
+        assert NextStep(b[0],b[1],evalInsStep((ICMP(config.ops["var_cmp"],sle,1,config.ops["var_x"],D(Int(0,IntType(1,false)))))));
+       
+        if dataToBool(OperandContents(b[1],config.ops["var_cmp"])){
+                        // assert ValidInstruction(b[1],(STORE(D(Int(0,IntType(1,false))),config.ops["var_retval"])));
+
+            assert NextStep(b[1],b[2],evalInsStep((STORE(D(Int(0,IntType(1,false))),config.ops["var_retval"]))));
+            // assert NextStep(b[2],b[3],evalInsStep((LOAD(config.ops["var_3"],1,config.ops["var_retval"]))));
+            // assert NextStep(b[3],b[4],evalInsStep((RET(config.ops["var_3"]))));
+
+        }else{
+            assert NextStep(b[1],b[2],evalInsStep((ICMP(config.ops["var_cmp1"],sgt,1,config.ops["var_x"],D(Int(2,IntType(1,false)))))));
+             if dataToBool(OperandContents(b[2],config.ops["var_cmp1"])){
+                    assert NextStep(b[2],b[3],evalInsStep((STORE(D(Int(0,IntType(1,false))),config.ops["var_retval"]))));
+             }else{
+                    assert NextStep(b[2],b[3],evalInsStep((STORE(config.ops["var_x"],config.ops["var_retval"]))));
+
+             }
+        }
+        assert last(b).o.Out?;
+        assert last(b).o.o.Int?;
+        assert last(b).o.o.val == 0 ||  last(b).o.o.val == 1 || last(b).o.o.val == 2;
+    }
+
+    lemma allVulnHaveIntOutput(s:State)
+        requires ValidState(s) 
+        requires validConfigVuln(s) 
+        // ensures last([s] + evalCodeFn(entryVuln(),s)).o.Out?;
+        // ensures last([s] + evalCodeFn(entryVuln(),s)).o.o.Int?;
+    {
+        var b_vuln := unwrapVuln(s);
+        // assert last([s] + evalCodeFn(entryVuln(),s)).o.Out?;
+        // assert forall s :: ValidState(s) && validConfigVuln(s) ==> last([s] + evalCodeFn(entryVuln(),s)).o.Out?;
+    }
+
+    lemma valsTest()
+        requires forall s :: (ValidState(s)  
+                            && validConfigVuln(s) 
+                            && (OperandContents(s,allVariablesConfigVuln().ops["var_x"]).val > 2
+                                || OperandContents(s,allVariablesConfigVuln().ops["var_x"]).val < 0))
+                            ==> (last([s] + evalCodeFn(entryVuln(),s)).o.Out?
+                                && last([s] + evalCodeFn(entryVuln(),s)).o.o.Int?
+                                && last([s] + evalCodeFn(entryPatch(),s)).o.Out?
+                                && last([s] + evalCodeFn(entryPatch(),s)).o.o.Int?
+                                && last([s] + evalCodeFn(entryVuln(),s)).o.o.val == last([s] + evalCodeFn(entryPatch(),s)).o.o.val)
+    {
+        reveal_ValidSimpleBehavior();
+        reveal_evalCodeFn();
+        forall s | ValidState(s) 
+                   && validConfigVuln(s)
+                   && OperandContents(s,allVariablesConfigVuln().ops["var_x"]).val <= 2
+                   && OperandContents(s,allVariablesConfigVuln().ops["var_x"]).val >= 0
+        {
+            var b_vuln := unwrapVuln(s);
+            var b_patch := unwrapPatch(s);
+
+            
+            assert exists s' :: last([s'] + evalCodeFn(entryVuln(),s')).o.o.val == 0;
+            // assert last(b_vuln).o.o.val == last(b_patch).o.o.val;
+            // assert last(b).o.o.val == 0 ||  last(b).o.o.val == 2 || last(b).o.o.val == 1;
+        }
+
+        // assert exists p,b :: ValidState(p) && validConfigVuln(p) && b == [p] + evalCodeFn(entryVuln(),p);
+    }
+
+}
