Dafny/examples/BenignTest/simpleTestBenign.i.dfy
@@ -1,0 +1,104 @@
+//make sure to add proper paths for the following..
+include "../../LLVM/llvmNEW.i.dfy"
+include "../../LLVM/types.s.dfy"
+
+module simpleTestBenign
+{
+	import opened LLVM_def_NEW
+	import opened types
+
+function allVariablesConfigVuln():Configuration
+{
+	var var_retval := LV("var_retval");
+	var var_cmp1 := LV("var_cmp1");
+	var var_3 := LV("var_3");
+	var var_cmp := LV("var_cmp");
+	var var_x := LV("var_x");
+	Config(map[
+		 "var_retval" := var_retval,
+		 "var_cmp1" := var_cmp1,
+		 "var_3" := var_3,
+		 "var_cmp" := var_cmp,
+		 "var_x" := var_x])
+}
+predicate validConfigVuln(s:State)
+	requires ValidState(s)
+{
+	var c := allVariablesConfigVuln(); 
+	&& (forall op :: op in c.ops ==> 
+		&& c.ops[op].LV? 
+		&& c.ops[op].l in s.lvs
+		&& ValidOperand(s,c.ops[op]))
+		 &&"var_retval" in c.ops
+		 &&"var_cmp1" in c.ops
+		 &&"var_3" in c.ops
+		 &&"var_cmp" in c.ops
+		 &&"var_x" in c.ops
+		//... add any additional state information
+
+		 && s.lvs["var_x"].Int?
+		 && s.lvs["var_x"].itype.size == 1
+		 && !s.lvs["var_x"].itype.signed
+		 && s.lvs["var_3"].Int?
+		 && s.lvs["var_retval"].Ptr?
+         && s.m.mem[OperandContents(s,c.ops["var_retval"]).bid][OperandContents(s,c.ops["var_retval"]).offset].mb? 
+         && s.m.mem[OperandContents(s,c.ops["var_retval"]).bid][OperandContents(s,c.ops["var_retval"]).offset].size == 1
+}
+
+function return_():Code{
+	var config := allVariablesConfigVuln();
+	var return_ := Block([Ins(LOAD(config.ops["var_3"],1,config.ops["var_retval"])),
+	Ins(RET(config.ops["var_3"]))]);
+	return_
+}
+
+function if_end():Code{
+	var config := allVariablesConfigVuln();
+	var if_end := Block([Ins(STORE(config.ops["var_x"],config.ops["var_retval"])),
+	return_()]);
+	if_end
+}
+
+function if_then():Code{
+	var config := allVariablesConfigVuln();
+	var if_then := Block([Ins(STORE(D(Int(0,IntType(1,false))),config.ops["var_retval"])),
+	return_()]);
+	if_then
+}
+
+function lor_lhs_false():Code{
+	var config := allVariablesConfigVuln();
+	var lor_lhs_false := Block([Ins(ICMP(config.ops["var_cmp1"],sgt,1,config.ops["var_x"],D(Int(2,IntType(1,false))))),
+	IfElse(config.ops["var_cmp1"],if_then(),if_end())]);
+	lor_lhs_false
+}
+
+function entryVuln():Code{
+	var config := allVariablesConfigVuln();
+	var entry := Block([Ins(ICMP(config.ops["var_cmp"],sle,1,config.ops["var_x"],D(Int(0,IntType(1,false))))),
+	IfElse(config.ops["var_cmp"],if_then(),lor_lhs_false())]);
+	entry
+}
+}
+
+
+// entry:
+//   %cmp = icmp sle i32 %x, 0
+//   br i1 %cmp, label %if.then, label %lor.lhs.false
+
+// lor.lhs.false:                                    ; preds = %entry
+//   %cmp1 = icmp sgt i32 %x, 2
+//   br i1 %cmp1, label %if.then, label %if.end
+
+// if.then:                                          ; preds = %lor.lhs.false, %entry
+//   store i32 0, i32* %retval, align 4
+//   br label %return
+
+// if.end:                                           ; preds = %lor.lhs.false
+//   store i32 %x, i32* %retval, align 4
+//   br label %return
+
+// return:                                           ; preds = %if.end, %if.then
+//   %3 = load i32, i32* %retval, align 4
+//   ret i32 %3
+  
