Dafny/examples/BenignTest/simpleTestPatchBenign.i.dfy
@@ -1,0 +1,52 @@
+//make sure to add proper paths for the following..
+include "../../LLVM/llvmNEW.i.dfy"
+include "../../LLVM/types.s.dfy"
+
+module simpleTestPatchBenign
+{
+	import opened LLVM_def_NEW
+	import opened types
+
+function allVariablesConfigPatch():Configuration
+{
+	var var_retval := LV("var_retval");
+	var var_cmp1 := LV("var_cmp1");
+	var var_3 := LV("var_3");
+	var var_cmp := LV("var_cmp");
+	var var_x := LV("var_x");
+	Config(map[
+		 "var_retval" := var_retval,
+		 "var_cmp1" := var_cmp1,
+		 "var_3" := var_3,
+		 "var_cmp" := var_cmp,
+		 "var_x" := var_x])
+}
+predicate validConfigPatch(s:State)
+	requires ValidState(s)
+{
+	var c := allVariablesConfigPatch(); 
+	&& (forall op :: op in c.ops ==> 
+		&& c.ops[op].LV? 
+		&& c.ops[op].l in s.lvs
+		&& ValidOperand(s,c.ops[op]))
+		 &&"var_retval" in c.ops
+		 &&"var_cmp1" in c.ops
+		 &&"var_3" in c.ops
+		 &&"var_cmp" in c.ops
+		 &&"var_x" in c.ops
+		//... add any additional state information
+
+		 && s.lvs["var_x"].Int?
+		 && s.lvs["var_x"].itype.size == 1
+		 && !s.lvs["var_x"].itype.signed
+		 && s.lvs["var_3"].Int?
+		 && s.lvs["var_retval"].Ptr?
+         && s.m.mem[OperandContents(s,c.ops["var_retval"]).bid][OperandContents(s,c.ops["var_retval"]).offset].mb? 
+         && s.m.mem[OperandContents(s,c.ops["var_retval"]).bid][OperandContents(s,c.ops["var_retval"]).offset].size == 1
+}
+function entryPatch():Code{
+	var config := allVariablesConfigPatch();
+	var entry := Block([Ins(RET(D(Int(0,IntType(4,false)))))]);
+	entry
+}
+}
