Dafny/examples/Challenge9/test.i.dfy
@@ -1,0 +1,35 @@
+include "Challenge9CodeExample.i.dfy"
+include "Challenge9PropertiesExample.i.dfy"
+include "../../LLVM/llvmNEW.i.dfy"
+include "../../LLVM/types.s.dfy"
+include "../../Libraries/Seqs.s.dfy"
+
+module a{
+    import opened challenge9CodeExample
+    import opened LLVM_def_NEW
+    import opened types
+    import opened Collections__Seqs_s
+    import opened challenge9PropertiesExample
+
+
+    lemma  vulnIs(s:State, b:Behavior)
+        requires ValidState(s) 
+        requires validConfig(s) 
+        requires b == [s] + evalCodeFn(entrySimplVuln(),s)
+               requires ValidOperand(last(b),allVariablesConfig().ops["var_28"])
+       requires OperandContents(last(b),allVariablesConfig().ops["var_28"]).Int?
+       requires ValidOperand(last(b),allVariablesConfig().ops["var_0"])
+       requires OperandContents(last(b),allVariablesConfig().ops["var_0"]).Int?
+        // ensures testVal(b)
+        // ensures badbehavior(s,b)
+        // ensures OperandContents(last(b),allVariablesConfig().ops["var_0"]).val >= 255 ==> miniSpec(s,b);
+    {
+        // vulnAlwaysReturns1();
+        var bVuln := unwrapVuln(s);
+        assert b == bVuln;
+        assert OperandContents(last(b),allVariablesConfig().ops["var_28"]).val == 1;  
+        assert OperandContents(last(b),allVariablesConfig().ops["var_0"]).val >= 255 ==> miniSpec(s,b);
+    }
+
+
+}
